Added an alternative statement of the prime theorem

Test/dafny4/Primes.dfy
@@ -18,6 +18,13 @@ lemma AlwaysMorePrimes(k: int)
   }
 }
 
+// Here is an alternative formulation of the theorem
+lemma NoFiniteSetContainsAllPrimes(s: set<int>)
+  ensures exists p :: IsPrime(p) && p !in s;
+{
+  AlwaysMorePrimes(if s == {} then 0 else PickLargest(s) + 1);
+}
+
 // ------------------------- lemmas and auxiliary definitions
 
 predicate AllPrimes(s: set<int>, bound: int)
@@ -49,7 +56,7 @@ lemma GetLargerPrime(s: set<int>, bound: int) returns (p: int)
 function product(s: set<int>): int
 {
   if s == {} then 1 else
-  var a := PickSmallest(s); a * product(s - {a})
+  var a := PickLargest(s); a * product(s - {a})
 }
 
 lemma product_property(s: set<int>)
@@ -84,13 +91,13 @@ lemma ProductPlusOneIsPrime(s: set<int>, q: int)
 
 // The following lemma is essentially just associativity and commutativity of multiplication.
 // To get this proof through, it is necessary to know that if x!=y and y==Pick...(s), then
-// also y==Pick...(s - {x}).  It is for this reason that we use PickSmallest, instead of
+// also y==Pick...(s - {x}).  It is for this reason that we use PickLargest, instead of
 // picking an arbitrary element from s.
 lemma RemoveFactor(x: int, s: set<int>)
   requires x in s;
   ensures product(s) == x * product(s - {x});
 {
-  var y := PickSmallest(s);
+  var y := PickLargest(s);
   if x != y {
     calc {
       product(s);
@@ -100,7 +107,7 @@ lemma RemoveFactor(x: int, s: set<int>)
       x * y * product(s - {y} - {x});
       { assert s - {y} - {x} == s - {x} - {y}; }
       x * y * product(s - {x} - {y});
-      { assert y == PickSmallest(s - {x}); }
+      { assert y == PickLargest(s - {x}); }
       x * product(s - {x});
     }
   }
@@ -162,58 +169,36 @@ lemma Composite(c: int) returns (a: int, b: int)
   }
 }
 
-function PickSmallest(s: set<int>): int
+function PickLargest(s: set<int>): int
   requires s != {};
 {
-  SmallestElementExists(s);
-  var x :| x in s && forall y :: y in s ==> x <= y;
+  LargestElementExists(s);
+  var x :| x in s && forall y :: y in s ==> y <= x;
   x
 }
 
-lemma SmallestElementExists(s: set<int>)
+lemma LargestElementExists(s: set<int>)
   requires s != {};
-  ensures exists x :: x in s && forall y :: y in s ==> x <= y;
+  ensures exists x :: x in s && forall y :: y in s ==> y <= x;
 {
   var s' := s;
   while true
     invariant s' != {} && s' <= s;
-    invariant forall x,y :: x in s' && y in s - s' ==> x <= y;
+    invariant forall x,y :: x in s' && y in s - s' ==> y <= x;
     decreases s';
   {
     var x :| x in s';  // pick something
-    if forall y :: y in s' ==> x <= y {
+    if forall y :: y in s' ==> y <= x {
       // good pick
       return;
     } else {
       // constrain the pick further
-      var y :| y in s' && y < x;
-      s' := set z | z in s && z < x;
+      var y :| y in s' && x < y;
+      s' := set z | z in s && x < z;
       assert y in s';
     }
   }
 }
-
-/*******  This might be an alternative way to implement PickSmallest, if one can prove the desired postcondition of this function  *******
-function PS(s: set<int>): int
-  requires s != {};
-{
-  NonEmptySet(s);  // TODO: why is this needed?
-  var x :| x in s;
-  if forall y :: y in s ==> x <= y then
-    x
-  else
-    var y :| y in s && y < x;  // since not all numbers in s are smaller than x, here is one that isn't
-    var s' := set m | m in s && m < x;  // this is the subset of s containing all numbers smaller than x
-    assert y in s';  // y is in that subset, which implies s' is nonempty
-    PS(s')
-}
-
-lemma NonEmptySet(s: set<int>)
-  requires s != {};
-  ensures exists y :: y in s;
-{
-}
-*******/
 
 // This axiom about % is needed.  Unfortunately, Z3 seems incapable of proving it.
 lemma MulDivMod(a: nat, b: nat, c: nat, j: nat)
